work on Clique, SAT, TSAT, LGraph

theories/L/Complexity/Problems/Clique.v
@@ -1,10 +1,10 @@
 From Undecidability.L Require Import L.
 From Undecidability.L.Tactics Require Import LTactics ComputableTactics.
 From Undecidability.L.Datatypes Require Import LProd LTerm LNat Lists LOptions.
-From Undecidability.L.Complexity Require Import NP Synthetic Monotonic.
+From Undecidability.L.Complexity Require Import NP Synthetic Monotonic LinTimeDecodable. 
 From Undecidability.L.Functions Require Import Size.
 
-From Undecidability.L.Datatypes Require Import LGraph. 
+From Undecidability.L.Datatypes Require Export LGraph. 
 
 
 (* k-Clique: duplicate-free list of k nodes such that all pairwise-distinct nodes are connected *)
@@ -15,3 +15,234 @@ Inductive isClique (g : UndirectedGraph) : list (Fin.t (V g)) -> nat -> Prop :=
 
 Definition Clique (input : UndirectedGraph * nat) :=
   let (g, k) := input in exists cl, @isClique g cl k. 
+
+Inductive isLClique (g : Lgraph) : list Lnode -> nat -> Prop :=
+| isLCliqueB : isLClique g [] 0
+| isLCliqueS (cl : list Lnode) (node : Lnode) (k : nat) : isLClique g cl k ->
+    (not (node el cl)) -> Lgraph_node_in_dec g node = true -> (forall (node' : Lnode), node' el cl -> Lgraph_edge_in_dec g node node' = true) -> isLClique g (node :: cl) (S k).                                                     
+
+Definition LClique (input : Lgraph * nat) :=
+  let (g, k) := input in exists cl, @isLClique g cl k. 
+
+Definition LClique_verifier (input : Lgraph * nat) (cert : term) :=
+  let (g, k) := input in 
+  exists (l : list nat),
+    cert = enc l /\ isLClique g l k. (*this includes that l is short enough*)
+
+Lemma isLClique_node_in (g : Lgraph) (k : nat) (cl : list Lnode) : isLClique g cl k -> forall n, n el cl -> Lgraph_node_in_dec g n = true. 
+Proof.
+  induction 1. 
+  -intros n [].
+  - intros n [-> | H3]. apply H1. now apply IHisLClique. 
+Qed. 
+
+Lemma isLClique_length (g : Lgraph) (k : nat) (cl : list Lnode) : isLClique g cl k -> k = (|cl|).
+Proof. induction 1; now cbn. Qed. 
+
+
+Lemma size_nat_enc_mono (n  :nat) (m : nat) :
+  n <= m -> size (enc n) <= size(enc m). 
+Proof. 
+  intros H; repeat rewrite size_nat_enc. lia. 
+Qed. 
+
+Section dupfree_dec.
+  Variable (X : Type).
+  Variable (eqbX : X -> X -> bool).
+  Variable (eqbX_correct : forall a b, a = b <-> eqbX a b = true). 
+
+  Fixpoint dupfreeb (l : list X) : bool :=
+    match l with [] => true
+            | (x :: ls) => negb (list_in_decb eqbX ls x) && dupfreeb ls
+  end. 
+
+  Lemma dupfreeb_correct (l : list X) : reflect (dupfree l) (dupfreeb l).
+  Proof.
+    destruct dupfreeb eqn:H; constructor. 
+    - induction l; constructor. all: cbn in H; apply andb_prop in H. 
+      all: cbn in H; destruct H. apply ssrbool.negbTE in H.
+      now intros H1%(list_in_decb_iff eqbX_correct).
+      now apply IHl.  
+    - intros H0. induction H0. cbn in H; congruence. 
+      apply IHdupfree. cbn in H; apply andb_false_elim in H. destruct H.
+      apply ssrbool.negbFE in e. apply (list_in_decb_iff eqbX_correct) in e. tauto. 
+      assumption. 
+  Qed.
+
+  Lemma dupfreeb_iff (l : list X) : dupfreeb l = true <-> dupfree l. 
+  Proof. 
+    specialize (dupfreeb_correct l) as H0.
+    destruct dupfreeb. inv H0. split; eauto. inv H0; split; eauto. 
+  Qed.
+
+End dupfree_dec. 
+
+Fixpoint connectedb (g : Lgraph) (cl : list Lnode) :=
+  match cl with [] => true
+           | (n :: cl) => forallb (Lgraph_edge_in_dec g n) cl && connectedb g cl
+  end. 
+
+(*TODO: maybe factor out the 2nd induction*)
+Lemma connectedb_correct (g : Lgraph) (cl : list Lnode) : dupfree cl -> connectedb g cl = true <-> forall u v, u <> v -> u el cl -> v el cl -> Lgraph_edge_in_dec g u v = true. 
+Proof. 
+  intros F0. 
+  destruct g. induction cl. 
+  + cbn. tauto. 
+  + split; cbn.
+  - intros H%andb_prop; destruct H as [F1 F2]. intros u v neq [H1 | H1] [H2 | H2].
+    * congruence.
+    * rewrite H1 in *; clear H1.
+      apply (proj1 (forallb_forall (Lgraph_edge_in_dec (n, l) u) cl) F1 v H2 ).
+    * rewrite H2 in *; clear H2.
+      specialize (proj1 (forallb_forall (Lgraph_edge_in_dec (n, l) v) cl) F1 u H1) as H0.
+      apply Lgraph_edge_in_dec'_correct. apply Lgraph_edge_in_dec'_correct in H0. tauto.
+    * inv F0. apply IHcl; tauto. 
+  - intros H. apply utils.andb_and; split.
+    2: {apply IHcl. firstorder. now inv F0. firstorder. }
+    clear IHcl. induction cl. reflexivity. 
+    cbn. apply utils.andb_and; split.
+    2: {inv F0. inv H3. assert (dupfree (a :: cl)). constructor. firstorder. apply H5. apply IHcl;firstorder. }
+    apply H. inv F0. 1-2: firstorder. right; left; reflexivity. 
+Qed. 
+
+Definition LClique_verifierb (g : Lgraph) (k : nat) (cl : list Lnode) :=
+  forallb (Lgraph_node_in_dec g) cl && dupfreeb Nat.eqb cl && connectedb g cl && Nat.eqb (|cl|) k.   
+
+Definition nat_eqb_correct := (fun a b => conj (proj2 (Nat.eqb_eq a b)) (proj1 (Nat.eqb_eq a b))). 
+
+Ltac simp_bool := repeat match goal with
+                  | [ H: negb (?b) = true , H' : ?b = true |- _] => rewrite negb_true_iff in H; congruence
+                  | [H : negb (?b) = false |- _] => apply ssrbool.negbFE in H; unfold is_true in H
+                  | [H : negb (?b) = true |- _] => apply ssrbool.negbTE in H
+                  | [ H : andb (?b1) (?b2) = true |- _] => apply andb_prop in H;
+                                                         let a := fresh "H" in
+                                                         let b := fresh "H" in
+                                                         destruct H as [a b]
+                  | [H : andb (?b1) (?b2) = false |- _] => apply andb_false_elim in H;
+                                                         destruct H as [H | H]
+                  | [H : false = andb (?b1) (?b2) |- _] => symmetry in H; simp_bool
+                  | [ |- context[andb (?b1) (?b2) = false]] => rewrite andb_false_iff 
+                  end; try congruence.
+
+Lemma LClique_verifierb_correct (g : Lgraph) (k : nat) (cl : list Lnode) :
+  reflect (isLClique g cl k) (LClique_verifierb g k cl). 
+Proof.
+  destruct LClique_verifierb eqn:H; constructor.
+  - unfold LClique_verifierb in H; simp_bool.
+    revert k H1; induction cl; intros k H1; cbn in H1; destruct k; try discriminate H1; constructor.
+    + apply IHcl.
+      * cbn in H0;simp_bool; tauto. 
+      * cbn in H3; simp_bool; tauto. 
+      * cbn in H2; simp_bool; tauto. 
+      * apply H1. 
+    + specialize (dupfreeb_correct nat_eqb_correct (a::cl)) as H; inv H.
+      -- symmetry in H4. simp_bool. intros H7.
+         apply (list_in_decb_iff nat_eqb_correct) in H7. congruence.
+      -- exfalso. simp_bool. cbn in H3; simp_bool. cbn in H3; simp_bool. 
+    + cbn in H0. simp_bool. 
+    + assert (dupfree (a::cl)) by ( now apply (proj1 (dupfreeb_iff nat_eqb_correct (a::cl)))).
+      specialize (connectedb_correct g H) as [H4 _]. specialize (H4 H2). 
+      intros b H5. apply H4. intros ->. now inv H. now left. now right. 
+  - intros H0; induction H0. now cbn in H. 
+    apply IHisLClique. clear IHisLClique. unfold LClique_verifierb in H.
+    simp_bool; cbn in H; simp_bool.
+    all: unfold LClique_verifierb; simp_bool; try tauto.
+    + apply (list_in_decb_iff) in H. tauto. apply nat_eqb_correct.   
+    + exfalso. specialize (forallb_forall (Lgraph_edge_in_dec g node) cl) as H4.
+      now apply H4 in H3.  
+Qed. 
+
+
+(*extraction of needed functions and derivation of runtime bounds in terms of encoding size*)
+
+Fixpoint dupfreeb_time (X : Type) (eqbT : X -> unit -> (nat * (X -> unit -> nat * unit ))) (l : list X) := match l with [] => 8 | l :: ls => list_in_decb_time eqbT ls l + 25 + dupfreeb_time eqbT ls end.
+Instance term_dupfreeb (X : Type) `{registered X}: computableTime' (@dupfreeb X) (fun eqb eqbT => (8, fun l _ => (dupfreeb_time eqbT l, tt))).
+Proof.
+  extract. 
+  solverec. 
+Defined. 
+
+Lemma dupfreeb_time_bound (X : Type) `{registered X} (eqbT : X -> unit -> (nat * (X -> unit -> nat * unit))):
+  (*eqbT is polynomial in encoding of a and b *)
+  (exists (f : nat -> nat), (forall (a b : X), callTime2 eqbT a b <= f (size(enc a) * size(enc b))) /\ inOPoly f)
+  -> exists (f : nat -> nat), (forall (l : list X), dupfreeb_time eqbT l <= f (size(enc l))) /\ inOPoly f. 
+Proof.
+  intros (f' & H1 & H2).  
+  evar (f : nat -> nat). exists f. split.
+  - intros l. unfold dupfreeb_time.  
+
+Definition forallb_time (X:Type) (fT : X -> unit -> nat * unit) (l : list X) := fold_right (fun elm acc => fst(fT elm tt) + acc + 15) 8 l.
+
+Instance term_forallb (X : Type) `{registered X} : computableTime' (@forallb X) (fun f fT => (1, fun l _ => (forallb_time fT l, tt))). 
+Proof.
+  extract. 
+  solverec. 
+  unfold forallb_time. solverec. 
+Defined. 
+
+  Fixpoint connectedb_time (g : Lgraph) (cl : list Lnode) :=
+    let (n, e) := g in 
+    match cl with [] => 4
+                | (cl :: cls) => forallb_time
+   (fun (v : Lnode) (_ : unit) =>
+    (list_in_decb_time pair_eqb_nat_time e (cl, v) +
+     list_in_decb_time pair_eqb_nat_time e (v, cl) + 29, tt)) cls + 19 + connectedb_time g cls
+              end. 
+
+Instance term_connectedb : computableTime' connectedb (fun g _ => (5, fun cl _ => (connectedb_time g cl, tt))).
+Proof.
+  extract. 
+  solverec. 
+Qed. 
+
+Definition Lclique_verifierb_time (g : Lgraph) (k:nat) (cl : list Lnode):= forallb_time (fun n _ => (33 + 14 * n, tt)) cl
+  + dupfreeb_time (fun x _ => (5, fun y _ => (min x y * 17 + 9, tt))) cl
+  + connectedb_time g cl + 11 * (|cl|) + 17 * min (|cl|) k + 53.
+Instance term_LClique_verifierb : computableTime' LClique_verifierb (fun g _ => (1, fun k _ => (1, fun cl _ => (Lclique_verifierb_time g k cl, tt)))). 
+Proof.
+  extract. 
+  solverec. unfold Lclique_verifierb_time. solverec. 
+Qed. 
+                 
+Lemma clique_inNP : inNP LClique. 
+Proof.
+  exists LClique_verifier. 
+  3 : {
+    intros [g k]; split.
+    - destruct g. intros (cert & H1). exists (enc cert), cert. split; try tauto.
+    - intros (ter & cert & H1 & H2). now exists cert. 
+  }
+  2 : {
+    evar (f' : nat -> nat). 
+    exists f'. split. 2: split. 
+    2: {
+      intros [g k] y (cert & H1 & H2).
+      assert (k = (|cert|)) by (now apply isLClique_length with (g:= g)).
+      rewrite H in *; clear H k. rewrite H1. rewrite size_prod; cbn [fst snd]. 
+      rewrite size_term_enc. rewrite size_nat_enc. rewrite size_list.   
+      recRel_prettify2.
+      (*LHS is in O(max_node * |cert|) *)
+      unfold Lgraph_node_in_dec in H2. destruct g.
+      assert (sumn (map (fun (x : nat ) => size (enc x) + 5) cert) <= (size(enc n) + 5) * (|cert|)). 
+      - clear H1. induction cert. cbn; lia.
+        cbn. assert (a <= n).
+        { assert (Lgraph_node_in_dec (n, l) a = true ).
+          apply isLClique_node_in with (k:= |a::cert|) (cl:= a::cert); easy.
+          cbn in H. destruct n. congruence. apply leb_complete in H. lia. 
+        } 
+        apply size_nat_enc_mono in H. rewrite H. rewrite IHcert. solverec. 
+        firstorder. now inv H2. 
+      - rewrite H. rewrite size_prod with (w := (n, l)); cbn [fst snd].
+        instantiate (f' := fun n => 4 * n * n). subst f'. 
+        solverec. 
+    }
+    all: (subst f'; smpl_inO). 
+  }
+
+  evar (f : nat -> nat). exists f. split; try split. 
+  - exists (fun inp => match inp with ((g, k), cert) => match decode (list nat) cert with Some cert => LClique_verifierb g k cert | _ => false end end).
+    split.
+    + constructor. extract. solverec.
+      repeat (rewrite size_prod; cbn [fst snd]).
+      unfold Lclique_verifierb_time. 
+Admitted. 
