theories/L/Complexity/Reductions/TSAT_to_SAT.v
@@ -1,0 +1,4 @@
+From Undecidability.L.Complexity Require Import NP Synthetic Problems.SAT Problems.Clique. 
+From Undecidability.L Require Import Tactics.LTactics.
+From Undecidability.L.Complexity Require Import Problems.TSAT. 
+
